Proofs/Rewrites.thy
@@ -75,7 +75,7 @@ proof -
     by (smt (z3) DiffI add_node_lookup replace_node_unchanged)
   then have c': "kind g' (nextNid g) = ConstantNode (IntVal32 1)"
     using truedef by simp
-  have "valid_value (constantAsStamp (IntVal32 1)) (IntVal32 1)"
+  have "valid_value (IntVal32 1) (constantAsStamp (IntVal32 1))"
     unfolding constantAsStamp.simps valid_value.simps
     using nat_numeral by blast
   then have "[g', m, p] \<turnstile> nextNid g \<mapsto> IntVal32 1"
@@ -103,7 +103,7 @@ proof -
     by (smt (z3) add_changed add_node_def assms(1) assms(2) constantCondition.simps(1) not_in_g other_node_unchanged replace_node_def replace_node_lookup singletonD)
   then have c': "kind g' (nextNid g) = ConstantNode (IntVal32 0)"
     using falsedef by simp
-  have "valid_value (constantAsStamp (IntVal32 0)) (IntVal32 0)"
+  have "valid_value (IntVal32 0) (constantAsStamp (IntVal32 0))"
     unfolding constantAsStamp.simps valid_value.simps
     using nat_numeral by blast
   then have "[g', m, p] \<turnstile> nextNid g \<mapsto> IntVal32 0"
